Working on conversion between [System] and [PSystem]

src/PredMsg.v
@@ -64,6 +64,20 @@ Inductive PRule :=
 | PRuleRqFwd: forall (rq: PMsgId) (prec: PRPrecond) (fwds: RqFwdF), PRule
 | PRuleRsBack: forall (rss: list PMsgId) (rsbf: RsBackF), PRule.
 
+Definition midsOfPRule (prule: PRule) :=
+  match prule with
+  | PRuleImm rq _ => pmid_mid rq :: nil
+  | PRuleRqFwd rq _ _ => pmid_mid rq :: nil
+  | PRuleRsBack rss _ => map pmid_mid rss
+  end.
+
+Definition precOfPRule (prule: PRule) :=
+  match prule with
+  | PRuleImm _ prec => prec
+  | PRuleRqFwd _ prec _ => prec
+  | PRuleRsBack _ _ => ⊤
+  end.
+
 Section PLabel.
 
   Inductive PLabel :=
@@ -94,6 +108,8 @@ Section PLabel.
   Definition emptyPLabel := PlblOuts None nil nil.
 
 End PLabel.
+
+Definition PHistory := list PLabel.
 
 Record PSystem :=
   { psys_inds: list IdxT;
@@ -133,109 +149,4 @@ Definition getPStateInit (psys: PSystem): PState :=
 Global Instance PSystem_PState_IsSystem : IsSystem PSystem PState :=
   {| indicesOf := psys_inds;
      initsOf := getPStateInit |}.
-
-Inductive step_pred (psys: PSystem): PState -> PLabel -> PState -> Prop :=
-| SpSlt: forall st, step_pred psys st emptyPLabel st
-
-| SpExt:
-    forall oss oims otrss (emsg: PMsg Rq),
-      isExternal psys (mid_from (msg_id (getMsg emsg))) = true ->
-      isInternal psys (mid_to (msg_id (getMsg emsg))) = true ->
-      step_pred psys
-                {| pst_oss := oss; pst_otrss := otrss; pst_msgs := oims |}
-                (PlblIn emsg)
-                {| pst_oss := oss;
-                   pst_otrss := otrss;
-                   pst_msgs := enqMP (existT _ _ emsg) oims
-                |}
-
-| SpImm:
-    forall oss oidx pos nos otrss oims (immr: PRule) prec (rq: PMsg Rq) (rs: PMsg Rs),
-      In oidx (indicesOf psys) ->
-      In immr (psys_rules psys) ->
-      immr = PRuleImm (pmsg_pmid rq) prec ->
-      DualPMsg rq rs ->
-      ValidMsgsIn oidx (rq :: nil) ->
-
-      oss@[oidx] = Some pos ->
-      prec pos (getMsg rq :: nil) ->
-      PredOk (pmsg_pred rq) (pmsg_val rq) (oss +[ oidx <- nos ]) (pmsg_val rs) ->
-
-      step_pred psys
-                {| pst_oss := oss; pst_otrss := otrss; pst_msgs := oims |}
-                (PlblOuts (Some immr)
-                          (existT _ _ rq :: nil)
-                          (existT _ _ rs :: nil))
-                {| pst_oss := oss +[ oidx <- nos ];
-                   pst_otrss := otrss;
-                   pst_msgs := distributeMsgs
-                                 (intOuts psys (existT _ _ rs :: nil))
-                                 (removeMP (existT _ _ rq) oims)
-                |}
-
-| SRqFwd:
-    forall oss otrss oidx pos opred rsbf oims (rqfwdr: PRule) prec outf
-           (rq: PMsg Rq) (fwds: list (PMsg Rq)) pred_ok,
-      In oidx (indicesOf psys) ->
-      In rqfwdr (psys_rules psys) ->
-      rqfwdr = PRuleRqFwd (pmsg_pmid rq) prec outf ->
-      ValidMsgsIn oidx (rq :: nil) ->
-      ValidMsgOuts oidx fwds ->
-
-      oss@[oidx] = Some pos ->
-      prec pos (getMsg rq :: nil) ->
-
-      step_pred psys
-                {| pst_oss := oss; pst_otrss := otrss; pst_msgs := oims |}
-                (PlblOuts (Some rqfwdr)
-                          (existT _ _ rq :: nil)
-                          (map (existT _ _) fwds))
-                {| pst_oss := oss;
-                   pst_otrss := otrss +[ oidx <- {| otrs_rq := rq;
-                                                    otrs_opred := opred;
-                                                    otrs_rsbf := rsbf;
-                                                    otrs_pred_ok := pred_ok |} ];
-                   pst_msgs := distributeMsgs
-                                 (map (existT _ _) fwds)
-                                 (removeMP (existT _ _ rq) oims)
-                |}
-
-| SRsBack:
-    forall oss otrss oidx pos nos otrs oims (rsbackr: PRule) rsbf
-           (rss: list (PMsg Rs)) (rsb: PMsg Rs),
-      In oidx (indicesOf psys) ->
-      In rsbackr (psys_rules psys) ->
-      rsbackr = PRuleRsBack (map (@pmsg_pmid _) rss) rsbf ->
-      ValidMsgsIn oidx rss ->
-      ValidMsgOuts oidx (rsb :: nil) ->
-
-      oss@[oidx] = Some pos ->
-      otrss@[oidx] = Some otrs ->
-
-      Forall (fun pmsg => PredOk
-                            (pmsg_pred pmsg)
-                            (pmsg_val (otrs_rq otrs)) oss (pmsg_val pmsg)) rss ->
-      otrs_opred otrs (pmsg_val (otrs_rq otrs)) nos (pmsg_val rsb) ->
-      otrs_rsbf otrs = rsbf ->
-      DualPMsg (otrs_rq otrs) rsb ->
-      pmsg_val rsb = rsbf (map getMsg rss) pos ->
-
-      step_pred psys
-                {| pst_oss := oss; pst_otrss := otrss; pst_msgs := oims |}
-                (PlblOuts (Some rsbackr)
-                          (map (existT _ _) rss)
-                          (existT _ _ rsb :: nil))
-                {| pst_oss := oss +[ oidx <- nos ];
-                   pst_otrss := M.remove oidx otrss;
-                   pst_msgs := enqMP (existT _ _ rsb)
-                                     (removeMsgs (map (existT _ _) rss) oims)
-                |}.
-
-Definition steps_pred: Steps PSystem PState PLabel := steps step_pred.
-
-(**
- * Informal TODOs:
- * 1) To prove [steps_det -> Transactional -> steps_pred]
- * 2) To check [steps_pred] is indeed useful for syntheses.
- *)
 
