src/PredMsgFacts.v
@@ -1,0 +1,28 @@
+Require Import Bool List String Peano_dec.
+Require Import Common FMap Syntax Semantics StepDet.
+Require Import PredMsg StepPred.
+Require Import Serial.
+
+(** Conversion from [PSystem] to [System] *)
+
+Definition pToRule (prule: PRule): Rule :=
+  {| rule_mids := midsOfPRule prule;
+     rule_precond := precOfPRule prule;
+     (** * TODO: how to convert? *)
+     rule_postcond := ⊤⊤⊤ |}.
+
+Definition pToSystem (psys: PSystem): System :=
+  {| sys_inds := psys_inds psys;
+     sys_inits := psys_inits psys;
+     sys_rules := map pToRule (psys_rules psys) |}.
+
+Theorem steps_pred_ok:
+  forall sys st1 thst st2 ts rqin mouts,
+    steps_det sys st1 thst st2 ->
+    Atomic sys ts rqin thst mouts ->
+    forall psys pst1 phst pst2,
+      pToSystem psys = sys ->
+      steps_pred psys pst1 phst pst2.
+Proof.
+Admitted.
+
